\documentclass{beamer}
\usetheme{Madrid}
% \usetheme{Frankfurt}
% \usetheme{Darmstadt}
% \usetheme{Berlin}
% \usetheme{Warsaw}
% \usetheme{Berkeley}
% \usetheme{Bergen}
% \usetheme{CambridgeUS}
% \usetheme{Copenhagen}

\providecommand{\pr}[1]{\ensuremath{\Pr\left(#1\right)}}
\providecommand{\cbrak}[1]{\ensuremath{\left\{#1\right\}}}
\newcommand{\mysolution}{\noindent \textbf{Solution: }}

\title{AI1110 - Probability and Random Variables\\
        Assignment 13}
\author{Aakash Kamuju (ai21btech11001)}
\begin{document}
\maketitle
    % \begin{frame}{Table of Contents}
    % \tableofcontents
    % \end{frame}
    \begin{frame}{Outline}
    \tableofcontents
    \end{frame}
    \begin{frame}{Question}
        \begin{section}{Question}
            \begin{block}{Example-15.24}
   Referring to the imbedded Markov chain formulation.
using the transition matrix the system of equations in $q_j = \Sigma q_jp_{ij}$ reduces to 
$$q_j = q_0 a_0 + \sum_{i=1} ^{j+1} q_i a_{j - i +1}$$.Then find Q(z)?
   \end{block}
    \end{section}
    \end{frame}
    \begin{frame}{Solution}
        \begin{section}{Solution}
            \begin{block}{Solution}
             $$Q(z) = \sum_{j = 0} ^{\infty} q_j z^j$$
              $$A(z) = \sum_{k = 0} ^{\infty} a_k z^k$$
              so by using the given equation, we get
        \end{block}
       \end{section}
  \end{frame}
  \begin{frame}
        \begin{section}{Solution}
            \begin{block}{Solution}
          $$Q(z)= q_0 \sum_{j = 0} ^{\infty} a_j z^j + \sum_{j = 0} ^{\infty} \sum_{i = 1} ^{j + 1}q_i a_{j-i+1} z^j$$
          $$Q(z) = q_0 A(z) + \sum_{i = 1} ^{\infty} q_i z^i \sum _{m = 0} ^{\infty} a_m z^m. z^{-1}$$
          $$Q(z) = q_0 A(Z) + (Q(z) - q_0)A(z)/z$$
          From this we get,

        \end{block}
       \end{section}
  \end{frame}
  \begin{frame}
        \begin{section}{Solution}
            \begin{block}{Solution}
           $$Q(z) = \frac{q_0(1 - z)A(z)}{A(z) - z}$$
        \end{block}
       \end{section}
  \end{frame}
   \end{document}
